Mostly done let-floating

03Debruijn/LetFloating.thy
@@ -1,5 +1,5 @@
 theory LetFloating
-  imports BigStep
+  imports Multisubst "../00Utils/Iteration" 
 begin
 
 subsection \<open>Let Floating\<close>
@@ -20,14 +20,25 @@ we can save ever executing these \<open>PopEnv\<^sub>e\<close>s. But we can do e
 text \<open>If we have an expression like \<open>App\<^sub>s (Let\<^sub>s e\<^sub>1\<^sub>1 e\<^sub>1\<^sub>2) e\<^sub>2\<close>, the above optimization will not apply; 
 the code for \<open>e\<^sub>2\<close> (and an \<open>Apply\<^sub>e\<close>) will sit between the \<open>PopEnv\<^sub>e\<close> and any eventual \<open>Return\<^sub>e\<close>. But 
 the expression \<open>Let\<^sub>s e\<^sub>1\<^sub>1 (App\<^sub>s e\<^sub>1\<^sub>2 (incr\<^sub>s 0 e\<^sub>2))\<close> has the same runtime behaviour - since we are in an 
-eagerly-evaluated language, all three subexpressions must be evaluated - but the scope of the \<open>Let\<^sub>s\<close> 
-now extends to the end of the expression. Similar transformations can be applied to 
-\<open>App\<^sub>s e\<^sub>1 (Let\<^sub>s e\<^sub>2\<^sub>1 e\<^sub>2\<^sub>2)\<close> and \<open>Let\<^sub>s (Let\<^sub>s e\<^sub>1\<^sub>1 e\<^sub>1\<^sub>2) e\<^sub>2\<close>, meaning that we can arrive at a form where every 
-lambda-expression is of the shape \<open>Lam\<^sub>s t (Let\<^sub>s e\<^sub>1 (... (Let\<^sub>s e\<^sub>n e) ...))\<close>, n \<ge> 0, and there are no 
-\<open>Let\<^sub>s\<close>s in any of the \<open>e\<close>s except under similarly-shaped lambda-expressions. (The top-level program 
-could in general not be a lambda-expression, but it will end with a \<open>Return\<^sub>e\<close> as well, so similar 
-remarks apply.) This means that _every_ \<open>PopEnv\<^sub>e\<close> will occur right before a \<open>Return\<^sub>e\<close>, and so can be 
-eliminated - and we can avoid compiling any code for \<open>PopEnv\<^sub>e\<close> at all.\<close>
+eagerly-evaluated language, all three subexpressions must be evaluated in the same order - but the 
+scope of the \<open>Let\<^sub>s\<close> now extends to the end of the expression. Similar transformations can be applied 
+to \<open>App\<^sub>s e\<^sub>1 (Let\<^sub>s e\<^sub>2\<^sub>1 e\<^sub>2\<^sub>2)\<close> and \<open>Let\<^sub>s (Let\<^sub>s e\<^sub>1\<^sub>1 e\<^sub>1\<^sub>2) e\<^sub>2\<close>, meaning that we can arrive at a form where 
+every lambda-expression is of the shape \<open>Lam\<^sub>s t (Let\<^sub>s e\<^sub>1 (... (Let\<^sub>s e\<^sub>n e) ...))\<close>, n \<ge> 0, and there 
+are no \<open>Let\<^sub>s\<close>s in any of the \<open>e\<close>s except under similarly-shaped lambda-expressions. (The top-level 
+program could in general not be a lambda-expression, but it will end with a \<open>Return\<^sub>e\<close> as well, so 
+similar remarks apply.) This means that _every_ \<open>PopEnv\<^sub>e\<close> will occur right before a \<open>Return\<^sub>e\<close>, and 
+so can be eliminated - and we can avoid compiling any code for \<open>PopEnv\<^sub>e\<close> at all.\<close>
+
+text \<open>There is one slight catch - naively floating the lets out of the argument of an application 
+\<open>App\<^sub>s e\<^sub>1 (Let\<^sub>s e\<^sub>2\<^sub>1 e\<^sub>2\<^sub>2)\<close> changes the evaluation order - before, \<open>e\<^sub>1\<close> is evaluated before \<open>e\<^sub>2\<^sub>1\<close>, but 
+once the latter has been floated out, it will be evaluated first. This is not necessarily fatal, 
+since our language is normalizing and has no side effects, but this would not extend to a richer 
+language, and would force us to work with big-step evaluation for proofs instead of the nicer 
+small-step relation. Fortunately, we can solve it another way: if \<open>e\<^sub>1\<close> is not a value, just let-bind 
+it too, thereby fixing the evaluation order. Because of our lifting of application left-sides, there 
+will be one extra evaluation step substituting it back away in each non-value \<open>App\<^sub>s\<close>, equivalent to 
+one extra \<open>Lookup\<^sub>e\<close> in the compiled tree-code. It will be made up for, hopefully, by the savings 
+from not having to pop the environments at the end of each function.\<close>
 
 text \<open>This transformation has one even more useful consequence, but it is not yet implemented - see
 the "Further Work" section at the end.\<close>
@@ -52,8 +63,15 @@ text \<open>Then, the let-floating transformation itself. We have to define a mu
 to make sure the variables match properly.\<close>
 
 primrec multiincr :: "nat \<Rightarrow> nat \<Rightarrow> expr\<^sub>d \<Rightarrow> expr\<^sub>d" where
-  "multiincr 0 y e = e"
-| "multiincr (Suc x) y e = incr\<^sub>d y (multiincr x y e)"
+  "multiincr 0 y = id"
+| "multiincr (Suc x) y = incr\<^sub>d y \<circ> multiincr x y"
+
+lemma multiincr_incr_absorb [simp]: "multiincr x y (incr\<^sub>d y e) = incr\<^sub>d y (multiincr x y e)"
+  by (induction x) simp_all
+
+lemma subst_multiincr_lemma [simp]: "(\<lambda>k. subst\<^sub>d (Suc (k + x)) (incr\<^sub>d y (multiincr k y e))) = 
+    ((\<lambda>k. subst\<^sub>d (k + x) (multiincr k y e)) \<circ> Suc)"
+  by auto
 
 fun strip_lets :: "expr\<^sub>d \<Rightarrow> expr\<^sub>d list \<times> expr\<^sub>d" where
   "strip_lets (Let\<^sub>d e\<^sub>1 e\<^sub>2) = (case strip_lets e\<^sub>2 of
@@ -65,19 +83,30 @@ primrec float_lets :: "expr\<^sub>d \<Rightarrow> expr\<^sub>d" where
 | "float_lets (Const\<^sub>d n) = Const\<^sub>d n"
 | "float_lets (Lam\<^sub>d t e) = Lam\<^sub>d t (float_lets e)"
 | "float_lets (App\<^sub>d e\<^sub>1 e\<^sub>2) = (case strip_lets (float_lets e\<^sub>1) of
-    (es\<^sub>1, e\<^sub>1') \<Rightarrow> (case strip_lets (multiincr (length es\<^sub>1) 0 (float_lets e\<^sub>2)) of
-      (es\<^sub>2, e\<^sub>2') \<Rightarrow> foldr Let\<^sub>d (es\<^sub>1 @ es\<^sub>2) (App\<^sub>d (multiincr (length es\<^sub>2) (length es\<^sub>1) e\<^sub>1') e\<^sub>2')))"
+    (es\<^sub>1, e\<^sub>1') \<Rightarrow> (case strip_lets (float_lets e\<^sub>2) of
+      (es\<^sub>2, e\<^sub>2') \<Rightarrow> 
+        let es\<^sub>1' = if value\<^sub>d e\<^sub>1' then es\<^sub>1 else es\<^sub>1 @ [e\<^sub>1']
+        in let e\<^sub>1'' = if value\<^sub>d e\<^sub>1' then e\<^sub>1' else Var\<^sub>d 0
+        in foldr Let\<^sub>d (es\<^sub>1' @ map_with_idx (multiincr (length es\<^sub>1')) es\<^sub>2) 
+            (App\<^sub>d (multiincr (length es\<^sub>2) 0 e\<^sub>1'') (multiincr (length es\<^sub>1') (length es\<^sub>2) e\<^sub>2'))))"
 | "float_lets (Let\<^sub>d e\<^sub>1 e\<^sub>2) = (case strip_lets (float_lets e\<^sub>1) of
     (es\<^sub>1, e\<^sub>1') \<Rightarrow> foldr Let\<^sub>d es\<^sub>1 (Let\<^sub>d e\<^sub>1' (multiincr (length es\<^sub>1) 1 (float_lets e\<^sub>2))))"
 
 lemma incr_let_free [simp]: "let_free (incr\<^sub>d x e) = let_free e"
   by (induction e arbitrary: x) simp_all
 
-lemma incr_let_floated [simp]: "let_floated (incr\<^sub>d x e) = let_floated e"
-  by (induction e arbitrary: x) simp_all
+lemma incr_let_free_map [simp]: "list_all let_free (map (incr\<^sub>d x) es) = list_all let_free es"
+  by (induction es) simp_all
 
 lemma multiincr_let_free [simp]: "let_free (multiincr x y e) = let_free e"
   by (induction x) simp_all
+
+lemma incr_let_floated [simp]: "let_floated (incr\<^sub>d x e) = let_floated e"
+  by (induction e arbitrary: x) simp_all
+
+lemma incr_let_floated_map [simp]: "list_all let_floated (map (incr\<^sub>d x) es) = 
+    list_all let_floated es"
+  by (induction es) simp_all
 
 lemma multiincr_let_floated [simp]: "let_floated (multiincr x y e) = let_floated e"
   by (induction x) simp_all
@@ -94,9 +123,9 @@ lemma float_lets_normalizes [simp]: "let_floated (float_lets e)"
 proof (induction e) 
   case (App\<^sub>d e1 e2)
   obtain es\<^sub>1 e\<^sub>1' where E1: "strip_lets (float_lets e1) = (es\<^sub>1, e\<^sub>1')" by fastforce
-  obtain es\<^sub>2 e\<^sub>2' where E2: "strip_lets (multiincr (length es\<^sub>1) 0 (float_lets e2)) = (es\<^sub>2, e\<^sub>2')" 
+  obtain es\<^sub>2 e\<^sub>2' where E2: "strip_lets (float_lets e2) = (es\<^sub>2, e\<^sub>2')" 
     by fastforce
-  from App\<^sub>d have "let_floated (multiincr (length es\<^sub>1) 0 (float_lets e2))" by simp
+  from App\<^sub>d have "let_floated (float_lets e2)" by simp
   with E2 have "list_all let_free es\<^sub>2 \<and> list_all let_floated es\<^sub>2 \<and> let_free e\<^sub>2' \<and> let_floated e\<^sub>2'" 
     by (metis strip_lets_normalized)
   with App\<^sub>d E1 E2 show ?case by simp
@@ -111,15 +140,58 @@ inductive typing\<^sub>d_bindings :: "ty list \<Rightarrow> expr\<^sub>d list \<
 inductive_cases [elim]: "\<Gamma> \<turnstile>\<^sub>d\<^sub>b [] : ts"
 inductive_cases [elim]: "\<Gamma> \<turnstile>\<^sub>d\<^sub>b e # es : ts"
 
+lemma typing_bindings_append [simp]: "\<Gamma> \<turnstile>\<^sub>d\<^sub>b es\<^sub>1 : ts\<^sub>1 \<Longrightarrow> ts\<^sub>1 @ \<Gamma> \<turnstile>\<^sub>d\<^sub>b es\<^sub>2 : ts\<^sub>2 \<Longrightarrow> 
+  \<Gamma> \<turnstile>\<^sub>d\<^sub>b es\<^sub>1 @ es\<^sub>2 : ts\<^sub>2 @ ts\<^sub>1"
+proof (induction es\<^sub>1 arbitrary: \<Gamma> ts\<^sub>1)
+  case (Cons e es\<^sub>1)
+  moreover then obtain t ts\<^sub>1' where T: "(\<Gamma> \<turnstile>\<^sub>d e : t) \<and> (insert_at 0 t \<Gamma> \<turnstile>\<^sub>d\<^sub>b es\<^sub>1 : ts\<^sub>1') \<and> 
+    ts\<^sub>1 = ts\<^sub>1' @ [t]" by fastforce
+  moreover with Cons have "ts\<^sub>1' @ insert_at 0 t \<Gamma> \<turnstile>\<^sub>d\<^sub>b es\<^sub>2 : ts\<^sub>2" by (induction \<Gamma>) simp_all
+  ultimately show ?case using tc\<^sub>d_bind_cons by fastforce
+qed auto
+
+lemma typing_bindings_eq_length [simp]: "\<Gamma> \<turnstile>\<^sub>d\<^sub>b es : ts \<Longrightarrow> length es = length ts"
+  by (induction \<Gamma> es ts rule: typing\<^sub>d_bindings.induct) simp_all
+
 lemma typing_multiincr [simp]: "\<Gamma>\<^sub>1 @ \<Gamma>\<^sub>2 \<turnstile>\<^sub>d e : t \<Longrightarrow> 
-    \<Gamma>\<^sub>1 @ \<Gamma>' @ \<Gamma>\<^sub>2 \<turnstile>\<^sub>d multiincr (length \<Gamma>') (length \<Gamma>\<^sub>1) e : t"
+  \<Gamma>\<^sub>1 @ \<Gamma>' @ \<Gamma>\<^sub>2 \<turnstile>\<^sub>d multiincr (length \<Gamma>') (length \<Gamma>\<^sub>1) e : t"
 proof (induction \<Gamma>')
   case (Cons tt \<Gamma>')
-  hence "insert_at (length \<Gamma>\<^sub>1) tt (\<Gamma>\<^sub>1 @ \<Gamma>' @ \<Gamma>\<^sub>2) \<turnstile>\<^sub>d 
-    incr\<^sub>d (length \<Gamma>\<^sub>1) (multiincr (length \<Gamma>') (length \<Gamma>\<^sub>1) e) : t" by simp
-  hence "\<Gamma>\<^sub>1 @ tt # \<Gamma>' @ \<Gamma>\<^sub>2 \<turnstile>\<^sub>d incr\<^sub>d (length \<Gamma>\<^sub>1) (multiincr (length \<Gamma>') (length \<Gamma>\<^sub>1) e) : t" try by simp
+  moreover have "length \<Gamma>\<^sub>1 \<le> length (\<Gamma>\<^sub>1 @ \<Gamma>' @ \<Gamma>\<^sub>2)" by simp
+  ultimately have "insert_at (length \<Gamma>\<^sub>1) tt (\<Gamma>\<^sub>1 @ \<Gamma>' @ \<Gamma>\<^sub>2) \<turnstile>\<^sub>d 
+    incr\<^sub>d (length \<Gamma>\<^sub>1) (multiincr (length \<Gamma>') (length \<Gamma>\<^sub>1) e) : t" by (metis tc\<^sub>d_incr)
   thus ?case by simp
 qed simp_all
+
+lemma typing_binding_incr [simp]: "\<Gamma>\<^sub>1 @ \<Gamma>\<^sub>2 \<turnstile>\<^sub>d\<^sub>b es : ts \<Longrightarrow> 
+  \<Gamma>\<^sub>1 @ t # \<Gamma>\<^sub>2 \<turnstile>\<^sub>d\<^sub>b map_with_idx (\<lambda>k. incr\<^sub>d (k + length \<Gamma>\<^sub>1)) es : ts" 
+proof (induction es arbitrary: \<Gamma>\<^sub>1 ts)
+  case (Cons e es)
+  then obtain ts' t' where T: "(\<Gamma>\<^sub>1 @ \<Gamma>\<^sub>2 \<turnstile>\<^sub>d e : t') \<and> (insert_at 0 t' (\<Gamma>\<^sub>1 @ \<Gamma>\<^sub>2) \<turnstile>\<^sub>d\<^sub>b es : ts') \<and> 
+    ts = ts' @ [t']" by fastforce
+  hence "insert_at 0 t' \<Gamma>\<^sub>1 @ \<Gamma>\<^sub>2 \<turnstile>\<^sub>d\<^sub>b es : ts'" by simp
+  with Cons have "insert_at 0 t' \<Gamma>\<^sub>1 @ t # \<Gamma>\<^sub>2 \<turnstile>\<^sub>d\<^sub>b 
+    map_with_idx (\<lambda>k. incr\<^sub>d (k + length (insert_at 0 t' \<Gamma>\<^sub>1))) es : ts'" by blast
+  hence X: "insert_at 0 t' (\<Gamma>\<^sub>1 @ t # \<Gamma>\<^sub>2) \<turnstile>\<^sub>d\<^sub>b 
+    map_with_idx ((\<lambda>k. incr\<^sub>d (k + length \<Gamma>\<^sub>1)) \<circ> Suc) es : ts'" by (simp add: comp_def)
+  from T have "insert_at (length \<Gamma>\<^sub>1) t (\<Gamma>\<^sub>1 @ \<Gamma>\<^sub>2) \<turnstile>\<^sub>d incr\<^sub>d (length \<Gamma>\<^sub>1) e : t'"
+    by (metis tc\<^sub>d_incr le_add1 length_append)
+  with T X show ?case by simp
+qed auto
+
+lemma typing_binding_multiincr [simp]: "\<Gamma>\<^sub>1 @ \<Gamma>\<^sub>2 \<turnstile>\<^sub>d\<^sub>b es : ts \<Longrightarrow> 
+  \<Gamma>\<^sub>1 @ \<Gamma>' @ \<Gamma>\<^sub>2 \<turnstile>\<^sub>d\<^sub>b map_with_idx (\<lambda>k. multiincr (length \<Gamma>') (k + length \<Gamma>\<^sub>1)) es : ts"
+proof (induction \<Gamma>')
+  case Nil
+  then show ?case by simp
+next
+  case (Cons t \<Gamma>')
+  hence "\<Gamma>\<^sub>1 @ t # \<Gamma>' @ \<Gamma>\<^sub>2 \<turnstile>\<^sub>d\<^sub>b map_with_idx (\<lambda>k. multiincr (Suc (length \<Gamma>')) (k + length \<Gamma>\<^sub>1)) es : 
+    ts" by simp
+  hence "\<Gamma>\<^sub>1 @ (t # \<Gamma>') @ \<Gamma>\<^sub>2 \<turnstile>\<^sub>d\<^sub>b map_with_idx (\<lambda>k. multiincr (length (t # \<Gamma>')) (k + length \<Gamma>\<^sub>1)) es : 
+    ts" by (simp del: multiincr.simps)
+  thus ?case by blast
+qed
 
 lemma typing_strip_lets [simp]: "\<Gamma> \<turnstile>\<^sub>d e : t \<Longrightarrow> strip_lets e = (es, e') \<Longrightarrow> 
   \<exists>ts. (\<Gamma> \<turnstile>\<^sub>d\<^sub>b es : ts) \<and> (ts @ \<Gamma> \<turnstile>\<^sub>d e' : t)"
@@ -149,34 +221,118 @@ next
   with tc\<^sub>d_let E X show ?case by auto
 qed
 
+lemma typing_fold_lets [simp]: "\<Gamma> \<turnstile>\<^sub>d\<^sub>b es : ts \<Longrightarrow> ts @ \<Gamma> \<turnstile>\<^sub>d e : t \<Longrightarrow> \<Gamma> \<turnstile>\<^sub>d foldr Let\<^sub>d es e : t"
+proof (induction \<Gamma> es ts rule: typing\<^sub>d_bindings.induct)
+  case (tc\<^sub>d_bind_cons \<Gamma> e t es ts)
+  thus ?case by (induction \<Gamma>) simp_all
+qed simp_all 
+
 theorem typing_float_lets [simp]: "\<Gamma> \<turnstile>\<^sub>d e : t \<Longrightarrow> \<Gamma> \<turnstile>\<^sub>d float_lets e : t"
 proof (induction \<Gamma> e t rule: typing\<^sub>d.induct)
   case (tc\<^sub>d_app \<Gamma> e\<^sub>1 t\<^sub>1 t\<^sub>2 e\<^sub>2)
   obtain es\<^sub>1 e\<^sub>1' where E1: "strip_lets (float_lets e\<^sub>1) = (es\<^sub>1, e\<^sub>1')" by fastforce
-  with tc\<^sub>d_app obtain ts\<^sub>1 where "(\<Gamma> \<turnstile>\<^sub>d\<^sub>b es\<^sub>1 : ts\<^sub>1) \<and> (ts\<^sub>1 @ \<Gamma> \<turnstile>\<^sub>d e\<^sub>1' : Arrow t\<^sub>1 t\<^sub>2)" by fastforce
-
-
-  obtain es\<^sub>2 e\<^sub>2' where E2: "strip_lets (multiincr (length es\<^sub>1) 0 (float_lets e\<^sub>2)) = (es\<^sub>2, e\<^sub>2')" by fastforce
-
+  with tc\<^sub>d_app obtain ts\<^sub>1 where T1: "(\<Gamma> \<turnstile>\<^sub>d\<^sub>b es\<^sub>1 : ts\<^sub>1) \<and> (ts\<^sub>1 @ \<Gamma> \<turnstile>\<^sub>d e\<^sub>1' : Arrow t\<^sub>1 t\<^sub>2)" by fastforce
+  let ?es\<^sub>1 = "if value\<^sub>d e\<^sub>1' then es\<^sub>1 else es\<^sub>1 @ [e\<^sub>1']"
+  let ?ts\<^sub>1 = "if value\<^sub>d e\<^sub>1' then ts\<^sub>1 else Arrow t\<^sub>1 t\<^sub>2 #  ts\<^sub>1"
+  let ?e\<^sub>1 = "if value\<^sub>d e\<^sub>1' then e\<^sub>1' else Var\<^sub>d 0"
   from tc\<^sub>d_app have "\<Gamma> \<turnstile>\<^sub>d float_lets e\<^sub>2 : t\<^sub>1" by simp
-  
-  
-  with tc\<^sub>d_app obtain ts\<^sub>2 where "(\<Gamma> \<turnstile>\<^sub>d\<^sub>b es\<^sub>2 : ts\<^sub>2) \<and> (ts\<^sub>2 @ \<Gamma> \<turnstile>\<^sub>d e\<^sub>2' : t\<^sub>1)" by fastforcex
-
-
-  from tc\<^sub>d_app have "\<Gamma> \<turnstile>\<^sub>d e\<^sub>1 : Arrow t\<^sub>1 t\<^sub>2" by simp
-  from tc\<^sub>d_app have "\<Gamma> \<turnstile>\<^sub>d e\<^sub>2 : t\<^sub>1" by simp
-  from tc\<^sub>d_app have "\<Gamma> \<turnstile>\<^sub>d float_lets e\<^sub>1 : Arrow t\<^sub>1 t\<^sub>2" by simp
-  from tc\<^sub>d_app have "\<Gamma> \<turnstile>\<^sub>d float_lets e\<^sub>2 : t\<^sub>1" by simp
-
-
-
-
-  have "\<Gamma> \<turnstile>\<^sub>d foldr Let\<^sub>d es\<^sub>1 (foldr Let\<^sub>d es\<^sub>2 (App\<^sub>d (multiincr (length es\<^sub>2) (length es\<^sub>1) e\<^sub>1') e\<^sub>2')) : t\<^sub>2" by simp
-  with E1 E2 show ?case by simp
+  moreover obtain es\<^sub>2 e\<^sub>2' where E2: "strip_lets (float_lets e\<^sub>2) = (es\<^sub>2, e\<^sub>2')" by fastforce
+  ultimately obtain ts\<^sub>2 where T2: "([] @ \<Gamma> \<turnstile>\<^sub>d\<^sub>b es\<^sub>2 : ts\<^sub>2) \<and> (ts\<^sub>2 @ \<Gamma> \<turnstile>\<^sub>d e\<^sub>2' : t\<^sub>1)" by fastforce
+  with T1 have L: "length ts\<^sub>1 = length es\<^sub>1 \<and> length ts\<^sub>2 = length es\<^sub>2" by auto
+  from T1 have "\<Gamma> \<turnstile>\<^sub>d\<^sub>b es\<^sub>1 @ [e\<^sub>1'] : [Arrow t\<^sub>1 t\<^sub>2] @ ts\<^sub>1"
+    by (metis append_Nil typing\<^sub>d_bindings.simps typing_bindings_append)
+  with T1 have X: "\<Gamma> \<turnstile>\<^sub>d\<^sub>b ?es\<^sub>1 : ?ts\<^sub>1" by simp
+  from T1 have "[] @ ?ts\<^sub>1 @ \<Gamma> \<turnstile>\<^sub>d ?e\<^sub>1 : Arrow t\<^sub>1 t\<^sub>2" by simp
+  hence Y: "[] @ ts\<^sub>2 @ ?ts\<^sub>1 @ \<Gamma> \<turnstile>\<^sub>d multiincr (length ts\<^sub>2) (length []) ?e\<^sub>1 : Arrow t\<^sub>1 t\<^sub>2" 
+    by (metis typing_multiincr list.size(3))
+  from T2 have Z: "[] @ ?ts\<^sub>1 @ \<Gamma> \<turnstile>\<^sub>d\<^sub>b map_with_idx (\<lambda>k. multiincr (length ?ts\<^sub>1) k) es\<^sub>2 : ts\<^sub>2" 
+    using typing_binding_multiincr by fastforce
+  from T2 have "ts\<^sub>2 @ ?ts\<^sub>1 @ \<Gamma> \<turnstile>\<^sub>d multiincr (length ?ts\<^sub>1) (length ts\<^sub>2) e\<^sub>2' : t\<^sub>1" by simp
+  with E1 E2 L X Y Z show ?case by (simp add: Let_def)
 next
   case (tc\<^sub>d_let \<Gamma> e\<^sub>1 t\<^sub>1 e\<^sub>2 t\<^sub>2)
-  then show ?case by simp
+  then obtain es\<^sub>1 e\<^sub>1' where E: "strip_lets (float_lets e\<^sub>1) = (es\<^sub>1, e\<^sub>1')" by fastforce
+  with tc\<^sub>d_let obtain ts\<^sub>1 where T1: "(\<Gamma> \<turnstile>\<^sub>d\<^sub>b es\<^sub>1 : ts\<^sub>1) \<and> (ts\<^sub>1 @ \<Gamma> \<turnstile>\<^sub>d e\<^sub>1' : t\<^sub>1)" by fastforce
+  hence L: "length ts\<^sub>1 = length es\<^sub>1" by auto
+  from tc\<^sub>d_let have "[t\<^sub>1] @ \<Gamma> \<turnstile>\<^sub>d float_lets e\<^sub>2 : t\<^sub>2" by (induction \<Gamma>) simp_all
+  hence "[t\<^sub>1] @ ts\<^sub>1 @ \<Gamma> \<turnstile>\<^sub>d multiincr (length ts\<^sub>1) (length [t\<^sub>1]) (float_lets e\<^sub>2) : t\<^sub>2" 
+    using typing_multiincr by fastforce
+  with L have "insert_at 0 t\<^sub>1 (ts\<^sub>1 @ \<Gamma>) \<turnstile>\<^sub>d multiincr (length es\<^sub>1) (Suc 0) (float_lets e\<^sub>2) : t\<^sub>2" 
+    by (cases "ts\<^sub>1 @ \<Gamma>") simp_all
+  with E T1 show ?case by auto
 qed simp_all
+
+lemma strip_lets_val [simp]: "value\<^sub>d v \<Longrightarrow> strip_lets v = ([], v)"
+  by (induction v) simp_all
+
+lemma foldr_let_val [simp]: "value\<^sub>d (foldr Let\<^sub>d es e) = (es = [] \<and> value\<^sub>d e)"
+  by (induction es) simp_all
+
+lemma float_lets_val [simp]: "value\<^sub>d (float_lets e) = value\<^sub>d e"
+  by (induction e) (auto split: prod.splits)
+
+lemma strip_lets_foldr [simp]: "strip_lets e = (es, e') \<Longrightarrow> foldr Let\<^sub>d es e' = e"
+  by (induction e arbitrary: es e') (auto split: prod.splits)
+
+lemma strip_lets_subst [simp]: "strip_lets e = (es, e') \<Longrightarrow> value\<^sub>d v \<Longrightarrow>
+    strip_lets (subst\<^sub>d x v e) = (map_with_idx (\<lambda>k. subst\<^sub>d (k + x) (multiincr k 0 v)) es, 
+      subst\<^sub>d (length es + x) (multiincr (length es) 0 v) e')"
+  by (induction e arbitrary: es x v) (auto split: prod.splits)
+
+lemma strip_lets_incr [simp]: "strip_lets e = (es, e') \<Longrightarrow> 
+    strip_lets (incr\<^sub>d x e) = (map_with_idx (\<lambda>k. incr\<^sub>d (k + x)) es, incr\<^sub>d (length es + x) e')"
+  by (induction e arbitrary: es x) (auto simp add: comp_def split: prod.splits)
+
+lemma foldr_let_incr [simp]: "incr\<^sub>d x (foldr Let\<^sub>d es e) = 
+    foldr Let\<^sub>d (map_with_idx (\<lambda>k. incr\<^sub>d (k + x)) es) (incr\<^sub>d (x + length es) e)"
+  by (induction es arbitrary: x) (simp_all add: comp_def)
+
+lemma float_lets_incr [simp]: "float_lets (incr\<^sub>d x e) = incr\<^sub>d x (float_lets e)"
+  apply (induction e arbitrary: x)
+      apply (simp_all split: prod.splits)
+  by simp
+
+lemma float_lets_subst [simp]: "float_lets (subst\<^sub>d x e' e) = subst\<^sub>d x (float_lets e') (float_lets e)"
+  apply (induction e arbitrary: x e')
+      apply (simp_allx split: prod.splits)
+  by simp
+
+theorem correctness\<^sub>f\<^sub>l [simp]: "e \<leadsto>\<^sub>d e' \<Longrightarrow> float_lets e \<leadsto>\<^sub>d float_lets e'"
+proof (induction e e' rule: eval\<^sub>d.induct)
+  case (ev\<^sub>d_app1 e\<^sub>1 e\<^sub>1' e\<^sub>2)
+  hence "float_lets e\<^sub>1 \<leadsto>\<^sub>d float_lets e\<^sub>1'" by simp
+
+  obtain xes\<^sub>1 xe\<^sub>1 where E1: "strip_lets (float_lets e\<^sub>1) = (xes\<^sub>1, xe\<^sub>1)" by fastforce
+  obtain xes\<^sub>2 xe\<^sub>2 where E2: "strip_lets (float_lets e\<^sub>2) = (xes\<^sub>2, xe\<^sub>2)" by fastforce
+
+  let ?xes\<^sub>1' = "if value\<^sub>d xe\<^sub>1 then xes\<^sub>1 else xes\<^sub>1 @ [xe\<^sub>1]"
+  let ?xe\<^sub>1 = "if value\<^sub>d xe\<^sub>1 then xe\<^sub>1 else Var\<^sub>d 0"
+
+  have "foldr Let\<^sub>d ?xes\<^sub>1' (foldr Let\<^sub>d (map_with_idx (multiincr (length ?xes\<^sub>1')) xes\<^sub>2)
+          (App\<^sub>d (multiincr (length xes\<^sub>2) 0 ?xe\<^sub>1) (multiincr (length ?xes\<^sub>1') (length xes\<^sub>2) xe\<^sub>2))) \<leadsto>\<^sub>d
+    (case strip_lets (float_lets e\<^sub>1') of
+     (xes\<^sub>1\<^sub>b, xe\<^sub>1') \<Rightarrow>
+         let xes\<^sub>1' = if value\<^sub>d xe\<^sub>1' then xes\<^sub>1\<^sub>b else xes\<^sub>1\<^sub>b @ [xe\<^sub>1']
+         in foldr Let\<^sub>d xes\<^sub>1'
+             (foldr Let\<^sub>d (map_with_idx (multiincr (length xes\<^sub>1')) xes\<^sub>2)
+               (App\<^sub>d (multiincr (length xes\<^sub>2) 0 (if value\<^sub>d xe\<^sub>1' then xe\<^sub>1' else Var\<^sub>d 0))
+                 (multiincr (length xes\<^sub>1') (length xes\<^sub>2) xe\<^sub>2))))" by simp
+  with E1 E2 show ?case by (simp add: Let_def)
+next
+  case (ev\<^sub>d_app2 e\<^sub>1 e\<^sub>2 e\<^sub>2')
+  then show ?case by simpx
+next
+  case (ev\<^sub>d_app3 e\<^sub>2 t e\<^sub>1)
+  then show ?case by simp
+next
+  case (ev\<^sub>d_let1 e\<^sub>1 e\<^sub>1' e\<^sub>2)
+  then show ?case by simpx
+next
+  case (ev\<^sub>d_let2 e\<^sub>1 e\<^sub>2)
+  then show ?case by simp
+qed
+
+lemma iter_correct\<^sub>f\<^sub>l [simp]: "iter (\<leadsto>\<^sub>d) e e' \<Longrightarrow> iter (\<leadsto>\<^sub>d) (float_lets e) (float_lets e')"
+  by simp
 
 end
